\documentclass{article}
\begin{document}

$S K K = (\lambda x. \lambda y. \lambda z.(x\ z\ (y\ z)))\ (\lambda x. \lambda y.x)\ (\lambda x. \lambda y.x)$

$\rightarrow_\beta (\lambda y. \lambda z.((\lambda x. \lambda y.x)\ z\ (y\ z)))\ (\lambda x. \lambda y.x)$

$\rightarrow_\beta \lambda z.((\lambda x. \lambda y.x)\ z\ (\lambda x. \lambda y.x)\ z)$

$\rightarrow_\beta \lambda z.((\lambda x. \lambda y.x)\ z\ (\lambda y.z))$

$\rightarrow_\beta \lambda z.((\lambda y.z)\ (\lambda y.z))$

$\rightarrow_\beta \lambda z.z = I$


\end{document}
